some additional facts for framing

Core/StatePredicates.v
@@ -46,6 +46,7 @@ Definition no_msg_from (from : nid) (d : soup) : Prop :=
 Definition no_msg_to (to : nid) (d : soup) : Prop :=
   forall i from tms b, find i d = Some (Msg tms from to b) -> b = false.
 
+
 Lemma no_msg_from_post (from from' to : nid) (s : soup) tms :
   valid s ->
   no_msg_from from s -> from' != from ->
@@ -283,4 +284,42 @@ rewrite D=>/mapP[z] I Z; subst x.
 by exists z.2; rewrite -surjective_pairing.
 Qed.
 
+(********************************************************)
+(*** More elaborated versions of the same predicates  ***)
+(********************************************************)
 
+Definition no_msg_from_to' from to
+           (criterion : nat -> seq nat -> bool) (d : soup) :=
+  forall i t c b,
+    find i d = Some (Msg (TMsg t c) from to b) ->
+    criterion t c ->
+    b = false.
+
+Lemma no_msg_from_to_consume' from to cond s i:
+  valid s ->
+  no_msg_from_to' from to cond s ->
+  no_msg_from_to' from to cond (consume_msg s i).
+Proof.
+move=>V H m t c b .
+rewrite /consume_msg; case: (find i s); last by move=>F; apply: (H m t c b F).
+move=>ms; case B: (m == i).
+- by move/eqP: B=>B; subst m; rewrite findU eqxx/= V; case. 
+by rewrite findU B/==>/(H m t c b).
+Qed.
+
+Lemma msg_spec_consume' s from to tg cnt cond i :
+  valid s -> 
+  find i s = Some {| content := TMsg tg cnt;
+                     from := from; to := to; active := true |} ->
+  msg_in_soup from to cond s ->
+  no_msg_from_to' from to cond (consume_msg s i).
+Proof.
+move=>V E[][j][[t][c]]F H1 H2. 
+move=>m t' c' b; rewrite /consume_msg; move: (find_some E).
+case: dom_find=>// msg->_ _; case B: (m == i).
+- by move/eqP: B=>B; subst m; rewrite findU eqxx/= V; case. 
+have X: j = i by apply: (H1 i); exists tg, cnt.
+subst j; rewrite findU B/=; case: b=>// E' _.
+suff X: i = m by subst i; rewrite eqxx in B.
+by apply: (H1 m); exists t', c'. 
+Qed.
